@prefix : <http://www.semanticweb.org/venkatre/ontologies/2023/5/common_metadata_ontology#> .
@prefix owl: <http://www.w3.org/2002/07/owl#> .
@prefix rdf: <http://www.w3.org/1999/02/22-rdf-syntax-ns#> .
@prefix xml: <http://www.w3.org/XML/1998/namespace> .
@prefix xsd: <http://www.w3.org/2001/XMLSchema#> .
@prefix rdfs: <http://www.w3.org/2000/01/rdf-schema#> .
@base <http://www.semanticweb.org/venkatre/ontologies/2023/5/common_metadata_ontology> .

<http://www.semanticweb.org/venkatre/ontologies/2023/5/common_metadata_ontology> rdf:type owl:Ontology .

#################################################################
#    Object Properties
#################################################################

###  http://www.semanticweb.org/venkatre/ontologies/2023/5/common_metadata_ontology#contains
:contains rdf:type owl:ObjectProperty ;
          rdfs:subPropertyOf owl:topObjectProperty ;
          rdfs:domain :Pipeline ;
          rdfs:range :Stages .


###  http://www.semanticweb.org/venkatre/ontologies/2023/5/common_metadata_ontology#executes
:executes rdf:type owl:ObjectProperty ;
          rdfs:subPropertyOf owl:topObjectProperty ;
          rdfs:domain :Pipeline ;
          rdfs:range :Task .


###  http://www.semanticweb.org/venkatre/ontologies/2023/5/common_metadata_ontology#generates
:generates rdf:type owl:ObjectProperty ;
           rdfs:subPropertyOf owl:topObjectProperty ;
           rdfs:domain :Execution ;
           rdfs:range :Metrics .


###  http://www.semanticweb.org/venkatre/ontologies/2023/5/common_metadata_ontology#has
:has rdf:type owl:ObjectProperty ;
     rdfs:subPropertyOf owl:topObjectProperty ;
     rdfs:domain :Pipeline ;
     rdfs:range :Framework ,
                :Report .


###  http://www.semanticweb.org/venkatre/ontologies/2023/5/common_metadata_ontology#isInput
:isInput rdf:type owl:ObjectProperty ;
         rdfs:subPropertyOf owl:topObjectProperty ;
         rdfs:domain :Artifacts ;
         rdfs:range :Execution .


###  http://www.semanticweb.org/venkatre/ontologies/2023/5/common_metadata_ontology#isOutput
:isOutput rdf:type owl:ObjectProperty ;
          rdfs:subPropertyOf owl:topObjectProperty ;
          rdfs:domain :Execution ;
          rdfs:range :Artifacts .


###  http://www.semanticweb.org/venkatre/ontologies/2023/5/common_metadata_ontology#run
:run rdf:type owl:ObjectProperty ;
     rdfs:subPropertyOf owl:topObjectProperty ;
     rdfs:domain :Stages ;
     rdfs:range :Execution .


###  http://www.semanticweb.org/venkatre/ontologies/2023/5/common_metadata_ontology#subCatof
:subCatof rdf:type owl:ObjectProperty ;
          rdfs:subPropertyOf owl:topObjectProperty ;
          rdfs:domain :Dataset ,
                      :Metrics ,
                      :Model ;
          rdfs:range :Artifacts .


###  http://www.semanticweb.org/venkatre/ontologies/2023/5/common_metadata_ontology#uses
:uses rdf:type owl:ObjectProperty ;
      rdfs:subPropertyOf owl:topObjectProperty ;
      rdfs:domain :Hyperparameters ;
      rdfs:range :Model .


#################################################################
#    Data properties
#################################################################

###  http://www.semanticweb.org/venkatre/ontologies/2023/5/common_metadata_ontology#abstract
:abstract rdf:type owl:DatatypeProperty ;
          rdfs:subPropertyOf owl:topDataProperty ;
          rdfs:domain :Report ;
          rdfs:comment "In some cases, the report can be a published paper which has an abstract. This property captures the abstract if available." .


###  http://www.semanticweb.org/venkatre/ontologies/2023/5/common_metadata_ontology#artifact_id
:artifact_id rdf:type owl:DatatypeProperty ;
             rdfs:subPropertyOf owl:topDataProperty ;
             rdfs:domain :Artifacts ,
                         :Dataset ,
                         :Model ;
             rdfs:comment "Unique ID generated for the artifacts produced as a result of execution" .


###  http://www.semanticweb.org/venkatre/ontologies/2023/5/common_metadata_ontology#artifact_name
:artifact_name rdf:type owl:DatatypeProperty ;
               rdfs:subPropertyOf owl:topDataProperty ;
               rdfs:domain :Artifacts ,
                           :Dataset ,
                           :Model ;
               rdfs:comment "Name of the artifact component - usually combination of pipeline name and execution name" .


###  http://www.semanticweb.org/venkatre/ontologies/2023/5/common_metadata_ontology#category
:category rdf:type owl:DatatypeProperty ;
          rdfs:subPropertyOf owl:topDataProperty ;
          rdfs:domain :Task ;
          rdfs:comment "The nature of the machine/deep learning task being performed such as detection, localization or summarization" .


###  http://www.semanticweb.org/venkatre/ontologies/2023/5/common_metadata_ontology#code_repo_url
:code_repo_url rdf:type owl:DatatypeProperty ;
               rdfs:subPropertyOf owl:topDataProperty ;
               rdfs:domain :Framework ;
               rdfs:comment "The URL to the code repository used to implement the pipeline" .


###  http://www.semanticweb.org/venkatre/ontologies/2023/5/common_metadata_ontology#command
:command rdf:type owl:DatatypeProperty ;
         rdfs:subPropertyOf owl:topDataProperty ;
         rdfs:domain :Execution ;
         rdfs:comment "Command Line Interface(CLI) command used to run the execution" .


###  http://www.semanticweb.org/venkatre/ontologies/2023/5/common_metadata_ontology#custom_properties
:custom_properties rdf:type owl:DatatypeProperty ;
                   rdfs:subPropertyOf owl:topDataProperty ;
                   rdfs:domain :Artifacts ,
                               :Dataset ,
                               :Execution ,
                               :Framework ,
                               :Hyperparameters ,
                               :Metrics ,
                               :Model ,
                               :Pipeline ,
                               :Report ,
                               :Stages ,
                               :Task ;
                   rdfs:comment "Custom Key-Value pairs that the user can add to capture more information about the compoenets of the pipeline" .


###  http://www.semanticweb.org/venkatre/ontologies/2023/5/common_metadata_ontology#dataset_id
:dataset_id rdf:type owl:DatatypeProperty ;
            rdfs:subPropertyOf owl:topDataProperty ;
            rdfs:domain :Dataset ;
            rdfs:comment "Unique ID for the dataset being used in the pipeline" .


###  http://www.semanticweb.org/venkatre/ontologies/2023/5/common_metadata_ontology#dataset_name
:dataset_name rdf:type owl:DatatypeProperty ;
              rdfs:subPropertyOf owl:topDataProperty ;
              rdfs:domain :Dataset ;
              rdfs:comment "Name of the dataset used for each execution of the pipeline" .


###  http://www.semanticweb.org/venkatre/ontologies/2023/5/common_metadata_ontology#dataset_url
:dataset_url rdf:type owl:DatatypeProperty ;
             rdfs:subPropertyOf owl:topDataProperty ;
             rdfs:domain :Dataset ;
             rdfs:comment "The public and official URL of the dataset from where the original data can be found along with documentation." .


###  http://www.semanticweb.org/venkatre/ontologies/2023/5/common_metadata_ontology#description
:description rdf:type owl:DatatypeProperty ;
             rdfs:subPropertyOf owl:topDataProperty ;
             rdfs:domain :Dataset ,
                         :Model ,
                         :Task ;
             rdfs:comment "Description of the components of the pipeline that provides additional information about the nodes" .


###  http://www.semanticweb.org/venkatre/ontologies/2023/5/common_metadata_ontology#execution_id
:execution_id rdf:type owl:DatatypeProperty ;
              rdfs:subPropertyOf owl:topDataProperty ;
              rdfs:domain :Artifacts ,
                          :Execution ;
              rdfs:comment "ID of the execution component" .


###  http://www.semanticweb.org/venkatre/ontologies/2023/5/common_metadata_ontology#execution_name
:execution_name rdf:type owl:DatatypeProperty ;
                rdfs:subPropertyOf owl:topDataProperty ;
                rdfs:domain :Execution ;
                rdfs:comment "Name of the various executions performed for each stage" .


###  http://www.semanticweb.org/venkatre/ontologies/2023/5/common_metadata_ontology#framework_id
:framework_id rdf:type owl:DatatypeProperty ;
              rdfs:subPropertyOf owl:topDataProperty ;
              rdfs:domain :Framework ;
              rdfs:comment "Unique ID for the framework being used" .


###  http://www.semanticweb.org/venkatre/ontologies/2023/5/common_metadata_ontology#framework_name
:framework_name rdf:type owl:DatatypeProperty ;
                rdfs:subPropertyOf owl:topDataProperty ;
                rdfs:domain :Framework ;
                rdfs:comment "Name of the framework being used to implement the pipeline" .


###  http://www.semanticweb.org/venkatre/ontologies/2023/5/common_metadata_ontology#metric_id
:metric_id rdf:type owl:DatatypeProperty ;
           rdfs:subPropertyOf owl:topDataProperty ;
           rdfs:domain :Metrics ;
           rdfs:comment "Unique ID for the metrics generated as a result of execution" .


###  http://www.semanticweb.org/venkatre/ontologies/2023/5/common_metadata_ontology#modality
:modality rdf:type owl:DatatypeProperty ;
          rdfs:subPropertyOf owl:topDataProperty ;
          rdfs:domain :Dataset ,
                      :Task ;
          rdfs:comment "The modality of the task and dataset such as image, text, audio or multimodal." .


###  http://www.semanticweb.org/venkatre/ontologies/2023/5/common_metadata_ontology#model_class
:model_class rdf:type owl:DatatypeProperty ;
             rdfs:subPropertyOf owl:topDataProperty ;
             rdfs:domain :Model ;
             rdfs:comment "The class of the models used in the pipeline such as CNN, GRU or Transformers" .


###  http://www.semanticweb.org/venkatre/ontologies/2023/5/common_metadata_ontology#model_id
:model_id rdf:type owl:DatatypeProperty ;
          rdfs:subPropertyOf owl:topDataProperty ;
          rdfs:comment "Unique ID for the models used in the pipeline" .


###  http://www.semanticweb.org/venkatre/ontologies/2023/5/common_metadata_ontology#param_id
:param_id rdf:type owl:DatatypeProperty ;
          rdfs:subPropertyOf owl:topDataProperty ;
          rdfs:domain :Hyperparameters ;
          rdfs:comment "Unique ID generated for the parameter settings used for each execution of the pipeline" .


###  http://www.semanticweb.org/venkatre/ontologies/2023/5/common_metadata_ontology#parameter_setting
:parameter_setting rdf:type owl:DatatypeProperty ;
                   rdfs:subPropertyOf owl:topDataProperty ;
                   rdfs:domain :Hyperparameters ;
                   rdfs:comment "A dict of parameter settings used for the models" .


###  http://www.semanticweb.org/venkatre/ontologies/2023/5/common_metadata_ontology#pdf_url
:pdf_url rdf:type owl:DatatypeProperty ;
         rdfs:subPropertyOf owl:topDataProperty ;
         rdfs:domain :Report ;
         rdfs:comment "PDF URL of the reports or published papers related to the pipeline" .


###  http://www.semanticweb.org/venkatre/ontologies/2023/5/common_metadata_ontology#pipeline_id
:pipeline_id rdf:type owl:DatatypeProperty ;
             rdfs:subPropertyOf owl:topDataProperty ;
             rdfs:comment "Unique ID generated for the pipelines" .


###  http://www.semanticweb.org/venkatre/ontologies/2023/5/common_metadata_ontology#pipeline_name
:pipeline_name rdf:type owl:DatatypeProperty ;
               rdfs:subPropertyOf owl:topDataProperty ;
               rdfs:domain :Artifacts ,
                           :Execution ,
                           :Pipeline ,
                           :Stages ;
               rdfs:comment "Name of the AI pipeline being executed" .


###  http://www.semanticweb.org/venkatre/ontologies/2023/5/common_metadata_ontology#report_id
:report_id rdf:type owl:DatatypeProperty ;
           rdfs:subPropertyOf owl:topDataProperty ;
           rdfs:comment "Unique ID generated for the report associated with the pipeline" .


###  http://www.semanticweb.org/venkatre/ontologies/2023/5/common_metadata_ontology#report_title
:report_title rdf:type owl:DatatypeProperty ;
              rdfs:subPropertyOf owl:topDataProperty ;
              rdfs:domain :Report ;
              rdfs:comment "Title of the report associated with the pipeline" .


###  http://www.semanticweb.org/venkatre/ontologies/2023/5/common_metadata_ontology#source
:source rdf:type owl:DatatypeProperty ;
        rdfs:subPropertyOf owl:topDataProperty ;
        rdfs:domain :Artifacts ,
                    :Dataset ,
                    :Execution ,
                    :Framework ,
                    :Hyperparameters ,
                    :Metrics ,
                    :Model ,
                    :Pipeline ,
                    :Report ,
                    :Stages ,
                    :Task ;
        rdfs:comment "The data source from where each of the nodes representing pipeline metadata are obtained." .


###  http://www.semanticweb.org/venkatre/ontologies/2023/5/common_metadata_ontology#source_id
:source_id rdf:type owl:DatatypeProperty ;
           rdfs:subPropertyOf owl:topDataProperty ;
           rdfs:domain :Dataset ,
                       :Metrics ,
                       :Model ,
                       :Pipeline ,
                       :Report ,
                       :Task ;
           rdfs:comment "The original ID that was given to the concept from their respective data sources." .


###  http://www.semanticweb.org/venkatre/ontologies/2023/5/common_metadata_ontology#stage_id
:stage_id rdf:type owl:DatatypeProperty ;
          rdfs:subPropertyOf owl:topDataProperty ;
          rdfs:domain :Execution ,
                      :Stages ;
          rdfs:comment "Unique ID for the stage component using UUID" .


###  http://www.semanticweb.org/venkatre/ontologies/2023/5/common_metadata_ontology#stage_name
:stage_name rdf:type owl:DatatypeProperty ;
            rdfs:subPropertyOf owl:topDataProperty ;
            rdfs:domain :Execution ,
                        :Stages ;
            rdfs:comment "Name of the AI pipeline stage that is being executed" .


###  http://www.semanticweb.org/venkatre/ontologies/2023/5/common_metadata_ontology#task_id
:task_id rdf:type owl:DatatypeProperty ;
         rdfs:subPropertyOf owl:topDataProperty ;
         rdfs:domain :Task ;
         rdfs:comment "Unique ID for the machine/deep learning task being performed by the pipeline" .


###  http://www.semanticweb.org/venkatre/ontologies/2023/5/common_metadata_ontology#task_name
:task_name rdf:type owl:DatatypeProperty ;
           rdfs:subPropertyOf owl:topDataProperty ;
           rdfs:domain :Task ;
           rdfs:comment "Name of the machine/deep learning task being executed" .


###  http://www.semanticweb.org/venkatre/ontologies/2023/5/common_metadata_ontology#task_type
:task_type rdf:type owl:DatatypeProperty ;
           rdfs:subPropertyOf owl:topDataProperty ;
           rdfs:domain :Task ;
           rdfs:comment "The type of machine learning task such as supervised learning, unsupervised learning or few-shot learning" .


###  http://www.semanticweb.org/venkatre/ontologies/2023/5/common_metadata_ontology#version
:version rdf:type owl:DatatypeProperty ;
         rdfs:subPropertyOf owl:topDataProperty ;
         rdfs:domain :Framework ;
         rdfs:comment "Version of the framework being used" .


#################################################################
#    Classes
#################################################################

###  http://www.semanticweb.org/venkatre/ontologies/2023/5/common_metadata_ontology#Artifacts
:Artifacts rdf:type owl:Class ;
           rdfs:comment "A list of artifacts that are produced as an output of execution or given as an input for an execution" .


###  http://www.semanticweb.org/venkatre/ontologies/2023/5/common_metadata_ontology#Dataset
:Dataset rdf:type owl:Class ;
         rdfs:comment "The dataset used for to execute a given task of a pipeline." .


###  http://www.semanticweb.org/venkatre/ontologies/2023/5/common_metadata_ontology#Execution
:Execution rdf:type owl:Class ;
           rdfs:comment "Various executions produced for a given stage. The stages could be feature engineering, training, evaluation and so on. Various executions can be produced for a given stage by executing the stage with different parameters" .


###  http://www.semanticweb.org/venkatre/ontologies/2023/5/common_metadata_ontology#Framework
:Framework rdf:type owl:Class ;
           rdfs:comment "Specifications of the framework with which the pipeline was implemented." .


###  http://www.semanticweb.org/venkatre/ontologies/2023/5/common_metadata_ontology#Hyperparameters
:Hyperparameters rdf:type owl:Class ;
                 rdfs:comment "The hyperparameters used for Model training" .


###  http://www.semanticweb.org/venkatre/ontologies/2023/5/common_metadata_ontology#Metrics
:Metrics rdf:type owl:Class ;
         rdfs:comment "Metrics is a subClassOf artifacts. Metrics are produced as an output of each execution" .


###  http://www.semanticweb.org/venkatre/ontologies/2023/5/common_metadata_ontology#Model
:Model rdf:type owl:Class ;
       rdfs:comment "Models used to train the pipeline. Also, the models produced as an output of an execution of a pipeline" .


###  http://www.semanticweb.org/venkatre/ontologies/2023/5/common_metadata_ontology#Pipeline
:Pipeline rdf:type owl:Class ;
          rdfs:comment "The AI pipeline that is being executed using the dataset, model and hyperparameters for a given task" .


###  http://www.semanticweb.org/venkatre/ontologies/2023/5/common_metadata_ontology#Report
:Report rdf:type owl:Class ;
        rdfs:comment "A report can be any documentation related to the pipeline. It can be published papers or readme" .


###  http://www.semanticweb.org/venkatre/ontologies/2023/5/common_metadata_ontology#Stages
:Stages rdf:type owl:Class ;
        rdfs:comment "The various stages of an AI pipeline such as data preprocessing, feature engineering, training, testing and so on." .


###  http://www.semanticweb.org/venkatre/ontologies/2023/5/common_metadata_ontology#Task
:Task rdf:type owl:Class ;
      rdfs:comment "The task for which the pipeline is being executed. For example, 3d object detection, 3d object segmentation and so on" .


#################################################################
#    General axioms
#################################################################

[ rdf:type owl:AllDisjointClasses ;
  owl:members ( :Artifacts
                :Dataset
                :Execution
                :Framework
                :Hyperparameters
                :Metrics
                :Model
                :Pipeline
                :Report
                :Stages
                :Task
              )
] .


###  Generated by the OWL API (version 4.5.9.2019-02-01T07:24:44Z) https://github.com/owlcs/owlapi
